Some working proofs

semantics/Semantic.v
@@ -186,34 +186,39 @@ Fixpoint read (st: state) (c: com) : locset :=
     | CAlloc (x) (mu) => LocSet.empty
     end.
 
-(* Inductive readR: state -> com -> locset -> Prop :=
+Inductive readR: state -> com -> state ->locset -> Prop :=
     | E_Read_CSkip:
-        forall st,
-        readR st CSkip (LocSet.empty)
+        forall st st',
+        st =[ skip ]=> (Some st') ->
+        readR st CSkip st' (LocSet.empty)
     | E_Read_CAsgn:
         forall st st' x a l,
+        st =[ x := a ]=> (Some st') ->
         upsilonR st a l ->
-        readR st <{ x := a }> l
-    | E_Read_CSeq st st' st'' c1 c2 l l' l'':
-        readR st c1 l1 ->
-        ceval st c1 = Some st' ->
-        readR st' c2 l2 ->
-        let lu := LocSet.union(l1 l2) in
-        readR st <{ c1 ; c2 }> .
+        readR st <{ x := a }> st' l
+    | E_Read_CSeq I1 M1 O1 c1 c2 R1 R2:
+        I1 =[ c1 ]=> (Some M1) ->
+        readR I1 c1 M1 R1 ->
+        M1 =[ c2 ]=> (Some O1) ->
+        readR M1 c2 O1 R2 ->
+        readR I1 <{ c1 ; c2 }> O1 (LocSet.union R1 R2).
 
-Inductive writeR: state -> locset -> com -> state -> locset -> Prop :=
-    | E_Write_CSkip st l:
-        writeR st l CSkip st l
+Inductive writeR: state -> com -> state -> locset -> Prop :=
+    | E_Write_CSkip st st':
+        st =[ skip ]=> (Some st') -> 
+        writeR st CSkip st' (LocSet.empty)
     | E_Write_CAsgn st st' l x a:
         st =[ x := a ]=> (Some st') -> 
-        writeR st l <{ x := a }> st' (LocSet.add (find_instance st x) l) 
-    | E_Write_CSeq st st' st'' c1 c2 l l' l'':
-        writeR st l c1 st' l' ->
-        writeR st' l' c2 st'' l'' ->
-        writeR st l <{ c1 ; c2 }> st'' l''. *)
+        writeR st <{ x := a }> st' (LocSet.add (find_instance st x) l) 
+    | E_Write_CSeq I1 M1 O1 c1 c2 W1 W2:
+        I1 =[ c1 ]=> (Some M1)->
+        writeR I1 c1 M1 W1 ->
+        M1 =[ c2 ]=> (Some O1) ->
+        writeR M1 c2 O1 W2 ->
+        writeR I1 <{ c1 ; c2 }> O1 (LocSet.union W1 W2).
 
 
-Inductive RW: state -> com -> locset -> locset -> Prop :=
+(* Inductive RW: state -> com -> locset -> locset -> Prop :=
     | E_RW_CSkip:
         forall st,
         RW st CSkip (LocSet.empty) (LocSet.empty)
@@ -228,10 +233,11 @@ Inductive RW: state -> com -> locset -> locset -> Prop :=
         cevalR c2 st' (Some st'') ->
         LocSet.Equal (LocSet.diff r2 w1) diff_r2_w1 ->
         LocSet.Equal (LocSet.union r1 diff_r2_w1) r ->
-        RW st <{ c1 ; c2 }> r w2.
+        RW st <{ c1 ; c2 }> r w2. *)
+
         
 
-Definition init_state := (W, 0) !-> VInt 10; _ !-> value.
+(* Definition init_state := (W, 0) !-> VInt 10; _ !-> value.
 Definition end_state := (W, 0) !-> VInt 10; (W, 0) !-> VInt 10; _ !-> value.
 Definition empty_set := LocSet.empty.
 Example test_readR_skip: 
@@ -265,7 +271,7 @@ Example test_readR_seq_asgn:
 Proof.
     intros * Heval1 Heval2.
     eapply E_RW_CSeq.
-Admitted.
+Admitted. *)
 
 Lemma LocSet_mem_1 : 
     forall l,
@@ -310,26 +316,370 @@ Lemma cevalR_det: forall c st1 st2 st,
     st1 = st2.
 Proof.
 Admitted.
+    
 
-Theorem rw_eval:
+Definition ten: Z := 10.
+
+Example test_readR_writeR_seq_asgn: 
+    forall x y R,
+    let st := empty_state in
+    let st'' := ((Y,0) !-> VInt 10; ((X,0) !-> VInt 10; empty_state)) in
+    readR st <{ x := ANum ten ; y := AId (X,0) }> st'' R ->
+    LocSet.Equal R (LocSet.singleton (X, 0)).
+Proof.
+    intros * Hread.
+    inversion Hread. subst.
+    inversion H2. inversion H9. subst.
+    inversion H7. subst. inversion H11. subst. easy.
+Qed.
+
+
+Definition find (v:MemMap.key) (st:MemMap.t value) := MemMap.find v st.
+
+
+Lemma no_change_outside_W:
+    forall c (I O: state) (W: locset),
+    writeR I c O W ->
+    (forall w, ~LocSet.In w W -> find w O = find w I).
+Proof.
+Admitted.
+
+
+Lemma LocSet_union_1:
+    forall l1 l2 l3,
+    LocSet.In l1 l2 -> LocSet.In l1 (LocSet.union l2 l3).
+Proof.
+    intros * H_in_l1.
+    apply FSetFact.union_iff. left. easy.
+Qed.
+
+Lemma LocSet_neg_union_1:
+    forall w W1 W2,
+    ~LocSet.In w W1 /\ ~LocSet.In w W2 <-> ~ LocSet.In w (LocSet.union W1 W2).
+Proof.
+Admitted.
+
+
+Lemma LocSet_union_non_disjoint:
+    forall l1 l2 l3,
+    LocSet.In l1 (LocSet.union l2 l3) <-> 
+    ((LocSet.In l1 l2 /\ LocSet.In l1 l3) \/
+    (LocSet.In l1 l2 /\ ~LocSet.In l1 l3) \/
+    (~LocSet.In l1 l2 /\ LocSet.In l1 l3)).
+Proof.
+Admitted.
+
+
+Lemma S_uses_only_R:
+    forall c (I1 O1 I2 O2: state) (R W: locset),
+    cevalR c I2 (Some O2) ->
+    readR I1 c O1 R ->
+    writeR I1 c O1 W ->
+    (forall r, LocSet.In r R -> find r I1 = find r I2) ->
+    (forall w, (LocSet.In w W -> find w O1 = find w O2) /\ (~LocSet.In w W -> find w O1 = find w I1 /\ find w O2 = find w I2)).
+Proof.
+    intros c.
+    (* remember c as c' eqn: Hc. *)
+    induction c.
+    (* Skip *)
+    -  intros * Hceval Hread Hwrite H_same_reads.
+        inversion Hceval. inversion Hread. inversion Hwrite. subst.
+        intros w.
+        split.
+        * intros H_in_w. easy.
+        * intros H_not_in_w. split; try easy. apply no_change_outside_W with (c:=<{ skip }>) (W:= LocSet.empty); try easy.
+
+
+    (* Seq *)
+    - intros * Hceval Hread Hwrite.
+        inversion Hceval as [|? M2|?|?|?|?]. inversion Hread. inversion Hwrite. subst.
+        assert (HM1: M0 = M1). admit. subst. clear H19. clear H16.
+
+        intros H_same_reads. intros w.
+
+        (* Do not depend on r2 M2 *)
+        assert (H_W_M1_M2: forall w, LocSet.In w W1 -> find w M1 = find w M2). {
+            intros * H_in_W1.
+            apply IHc1 with (I1:=I1) (O1:=M1) (I2:=I2) (O2:=M2) (R:=R1) (W:=W1); try easy.
+            intros r. specialize (H_same_reads r). intros H_in_R1. apply H_same_reads. rewrite FSetFact.union_iff. left. easy.
+        }
+
+        (* Do not depend on r2 M2 *)
+        assert (H_W1_not_W2_M1_M2: forall w, LocSet.In w W1 /\ ~ LocSet.In w W2 -> find w M1 = find w M2). {
+            intros.
+            apply H_W_M1_M2. easy.
+        }
+    
+
+        (* I1 = M1 /\ I2 = M2 /\ I1 = I2  *)
+(* 
+        assert (H_not_W1: forall r, LocSet.In r R2 -> ~ LocSet.In r W1 -> find r M1 = find r I1 /\ find r M2 = find r I2). admit.
+        assert (H_W1: forall r, LocSet.In r R2 -> LocSet.In r W1 -> find r M1 = find r M2). admit. *)
+
+        assert (H_R2_not_W1: forall r, ~LocSet.In w W1 /\ LocSet.In r R2 -> find r M1 = find r M2). {
+            admit.
+        }
+
+        assert (H_R2_W1: forall r, LocSet.In w W1 /\ LocSet.In r R2 -> find r M1 = find r M2). {
+            admit.
+        }
+
+        assert (H_not_W1_W2: ~ LocSet.In w W1 /\ LocSet.In w W2 -> find w O1 = find w O2). {
+            intros.
+            destruct H1.
+            apply IHc2 with (I1:=M1) (O1:=O1) (I2:=M2) (O2:=O2) (R:=R2) (W:=W2); try easy.
+            intros r.
+            intro H_in_R2. 
+            apply H_R2_not_W1; try easy.
+        }
+
+        assert (H_W1_not_W2_O1_M1: LocSet.In w W1 /\ ~ LocSet.In w W2 -> find w O1 = find w M1 /\ find w O2 = find w M2). {
+            intros H3.
+            destruct H3.
+            apply IHc2 with (I1:=M1) (O1:=O1) (I2:=M2) (O2:=O2) (R:=R2) (W:=W2); try easy.
+            intros r.
+            intro H_in_R2.
+            apply H_R2_W1; try easy.
+        }
+
+        assert (H_W1_not_W2:
+        ((find w M1 = find w M2) /\ (find w O1 = find w M1) /\ (find w O2 = find w M2))  ->
+        find w O1 = find w O2). {
+            intros H3.
+            destruct H3.
+            destruct H2.
+            rewrite H1 in H2.
+            apply transitivity with (x:=find w O1) (y:=find w M2) (z:=find w O2); try easy.
+        }
+
+
+
+        split.
+
+(* In W1 U W2 *)
+        *  
+        intros H_in_W.
+            rewrite LocSet_union_non_disjoint in H_in_W.
+            destruct H_in_W.
+            -- destruct H1. apply IHc2 with (I1:=M1) (O1:=O1) (I2:=M2) (O2:=O2) (R:=R2) (W:=W2); try easy.
+                intros r.
+                intro H_in_R2.
+                apply H_R2_W1; try easy.
+            -- destruct H1.
+                ++ apply H_W1_not_W2.
+                   split.
+                    ** apply H_W1_not_W2_M1_M2. easy.
+                    ** apply H_W1_not_W2_O1_M1. easy.
+                ++ apply H_not_W1_W2. easy.
+                (* ++ apply H_not_W1_W2; try easy. *)
+(* 
+        * intros H_not_in_W. rewrite <- LocSet_neg_union_1 in H_not_in_W.
+            assert (H_not_W1: ~LocSet.In w W1 /\ ~LocSet.In w W2 -> find w O1 = find w I1). admit.
+            assert (H_not_W2: ~LocSet.In w W1 /\ ~LocSet.In w W2 -> find w O2 = find w I2). admit.
+            split.
+            -- apply H_not_W1. easy.
+            -- apply H_not_W2. easy. *)
+
+(* 
+
+        assert (H_W1: LocSet.In w W1 -> find w O1 = find w O2).
+        {
+            intros H_in_W1.
+            admit.
+        }
+        assert (H_W2: LocSet.In w W2 -> find w O1 = find w O2). admit.
+
+
+
+        (* w in W1 U W2  or w notin*)
+        split.
+        * intros H_in_W. rewrite FSetFact.union_iff in H_in_W. destruct H_in_W as [H_in_W1 | H_in_W2].
+            -- apply H_W1. easy.
+            -- apply H_W2. easy.
+        *  *)
+
+        
+
+
+            
+
+    
+
+
+
+(* assert (H_EQ_O1_O2: forall w, 
+LocSet.In w W1 -> 
+    (LocSet.In w R1 -> (LocSet.In w W1 -> find w M1 = find w M2) \/ (~LocSet.In w W1 -> find w M1 = find w M2)) 
+    \/ 
+    (LocSet.In w R2 -> (LocSet.In w W2 -> find w O1 = find w O2) \/ (~LocSet.In w W2 -> find w O1 = find w O2))
+). admit. *)
+            
+    (* apply H_EQ_O1_O2.  *)
+
+           
+        
+            
+
+
+        (* specialize IHc1 with (I1:=I1) (O1:=M1) (I2:=I2) (O2:=M2) (R:=R1) (W:=W1) as IHc1'. *)
+(* 
+        assert (H_R1_W1_M1_M2: forall w, (LocSet.In w W1 -> find w M1 = find w M2) /\ (~LocSet.In w W1 -> find w M1 = find w I1 /\ find w M2 = find w I2)). {
+            apply IHc1 with (R:=R1); try easy.
+            intros r. specialize (H_same_reads r). intros H_in_R1. apply H_same_reads. rewrite FSetFact.union_iff. left. easy.
+        }
+
+        assert (H_R2_W2_O1_O2: forall w, (LocSet.In w W2 -> find w O1 = find w O2) /\ (~LocSet.In w W2 -> find w O1 = find w M1 /\ find w O2 = find w M2)). {
+            apply IHc2 with (R:=R2); try easy.
+            intros r. specialize (H_same_reads r). intros H_in_R2. apply H_R1_W1_M1_M2.
+            admit.
+        }
+
+        assert (HQ: forall r, (LocSet.In r R2 -> (LocSet.In r W1 -> find r M1 = find r M2) /\ (~LocSet.In r W1 -> find r M1 = find r I1 /\ find r I2 = find r M2 /\ find r I1 = find r I2))). {
+            intros r H_in_R2.
+            split.
+            * admit.
+            * intros H_not_in_W1. split.
+            (* r notin W1 *)
+              -- admit.
+              -- split.
+                 (* I2 = M2 on r *)
+                ++ admit.
+                (* I1 = I2 on r  *)
+                ++ apply H_same_reads. rewrite FSetFact.union_iff. right. easy.
+        }
+
+
+        assert (HR: forall r, (LocSet.In r R2 -> (LocSet.In r W2 -> find r O1 = find r O2) /\ (~LocSet.In r W2 -> find r O1 = find r M1 /\ find r O2 = find r M2 /\ find r M1 = find r M2))). { 
+            intros r H_in_R2.
+            split; try easy.
+            - apply H_R2_W2_O1_O2.
+            - intros H_not_in_W2. split.
+                + apply H_R2_W2_O1_O2; try easy.
+                + split.
+                   * apply H_R2_W2_O1_O2; try easy.
+                   * apply 
+        }
+
+        split.
+        * intros H_in_W. rewrite FSetFact.union_iff in H_in_W. destruct H_in_W as [H_in_W1 | H_in_W2].
+            -- 
+           *)
+
+
+
+        (* intros H_same_r w. split.
+        * intros H_in_w.
+          apply FSetFact.union_iff in H_in_r.
+          apply FSetFact.union_iff in H_in_w.
+          
+
+        * intros H_not_in_w.
+          admit. *)
+
+        (* inversion Hceval. inversion Hread. inversion Hwrite. subst.
+
+        assert (Hst1: st'0 = st'1). admit. subst. clear H19.
+
+        assert (H_r1_w1: forall r, LocSet.In r r1 -> MemMap.find r st1 = MemMap.find r st2 -> forall w, LocSet.In w w1-> MemMap.find w st1' = MemMap.find w st2'). {   
+            admit.
+        }
+        
+        assert (H_r2_w2: forall r, LocSet.In r r2 -> MemMap.find r st1 = MemMap.find r st2 -> forall w, LocSet.In w w2 -> MemMap.find w st1' = MemMap.find w st2'). {
+            admit.
+        }
+
+        assert (H_r1_w2: forall r, LocSet.In r r1 -> MemMap.find r st1 = MemMap.find r st2 -> forall w, LocSet.In w w2 -> MemMap.find w st1' = MemMap.find w st2'). {
+            admit.
+        }
+
+        assert (H_r2_w1: forall r, LocSet.In r r2 -> MemMap.find r st1 = MemMap.find r st2 -> forall w, LocSet.In w w1 -> MemMap.find w st1' = MemMap.find w st2'). {
+            admit.
+        }
+
+        intros * H_in_r H_same_r w H_in_w.
+
+        rewrite FSetFact.union_iff in *.
+        
+        destruct H_in_r as [H_in_R1 | H_in_R2];  destruct H_in_w as [H_in_W1 | H_in_W2].
+        (* r in R1 *) (* w in W1 *)
+        * apply H_r1_w1 with (r:=r); try easy.
+            
+        (* r in R1 *) (* w in W2 *)
+        * apply H_r1_w2 with (r:=r); try easy.
+
+        (* r in R2 *) (* w in W1 *) 
+        * apply H_r2_w1 with (r:=r); try easy.
+
+        (* r in R2 *) (* w in W2 *)
+        * apply H_r2_w2 with (r:=r); try easy. *)
+Admitted.
+        
+        (* * specialize IHc1 with (st1:=st1) (st2:=st2) (st1':=st'1) (st2':=st'2) (R:=l1) (W:=l4) as IHc1'.
+          specialize IHc2 with (st1:=st'1) (st2:=st'2) (st1':= st1') (st2':=st2') (R:=l2) (W:=l7) as IHc2'. *)
+
+
+
+      
+
+       
+      
+    
+    (* intros * Hread1 Hread2 Hwrite1 Hwrite2 H_eq_R H_eq_W H_eq_on_R.
+      inversion Hread1. inversion Hread2. inversion Hwrite1. inversion Hwrite2. subst.
+
+
+      assert (Hst1: st' = st'1). apply cevalR_det with (c:=c1) (st:=st1) (st1:=st') (st2:=st'1); easy. subst. clear H19. clear H22. 
+      assert (Hst2: st'0 = st'2). apply cevalR_det with (c:=c1) (st:=st2) (st1:=st'0) (st2:=st'2); easy. subst. clear H28. clear H31.
+         
+
+      assert (Hw: forall w, LocSet.In w (LocSet.union l4 l6) -> MemMap.find w st'1 = MemMap.find w st'2). admit.
+        
+      specialize (IHc2 st'1 st'2 st1' st2' l2 l3 (LocSet.union l4 l5) l7) as IHc2'.
+      apply IHc2'; try easy. *)
+      
+
+
+(* Theorem rw_eval:
 forall c st1 st1' st2 st2' reads writes,
 RW st1 c reads writes ->
 cevalR c st1 (Some st1') ->
 cevalR c st2 (Some st2') ->
-(forall l, LocSet.In l reads -> MemMap.find l st1 = MemMap.find l st2) ->
-(forall l, LocSet.In l writes -> MemMap.find l st1' = MemMap.find l st2').
+(forall r, LocSet.In r reads -> MemMap.find r st1 = MemMap.find r st2) ->
+(forall w, LocSet.In w writes -> MemMap.find w st1' = MemMap.find w st2').
 Proof.
     intros c.
-    induction c; intros * Hrw Hceval1 Hceval2;  try easy.
+    induction c; intros * Hrw Hceval1 Hceval2 Hsamereads;  try easy.
     - inversion Hceval1. inversion Hceval2. inversion Hrw. subst.
-      intros Hsamereads. intros l. easy.
+      intros l. easy.
     - inversion Hceval1. inversion Hceval2. inversion Hrw. subst.
-      intros Hsamereads.
 
       assert (Hst1: st' = st'1). apply cevalR_det with (c:=c1) (st:=st1) (st1:=st') (st2:=st'1); easy. subst. clear H14.
       assert (Hst1: st1' = st''1). apply cevalR_det with (c:=c2) (st:=st'1) (st1:=st1') (st2:=st''1); easy. subst. clear H16.
+         
+
+      assert (Hst1': forall w , LocSet.In w writes -> MemMap.find w st'1 = MemMap.find w st'0). admit.
 
 
+
+      specialize (IHc2 st'1 st''1 st'0 st2' r2 writes) as IHC2'.
+      specialize (IHc1 st1 st'1 st2 st'0 r1 w1) as IHc1'.
+       (* admit. *)
+
+    - inversion Hceval1. inversion Hceval2. inversion Hrw. subst.
+        unfold find_instance in *.
+        induction a; try easy.
+        (* a = n *)
+        * inversion H14. subst. inversion H2. subst. inversion H7. subst.
+            intros l. intro Hinl. rewrite LocSet_singleton_iff in Hinl. subst.
+            rewrite MemMap_find_1. rewrite MemMap_find_1. easy.
+        (* a = l *)
+        * inversion H14. subst. inversion H2. subst. inversion H7. subst.
+            specialize (Hsamereads l).
+            intros l0. intro Hinl0. rewrite LocSet_singleton_iff in Hinl0. subst.
+            rewrite MemMap_find_1. rewrite MemMap_find_1.
+            rewrite LocSet_singleton_iff in Hsamereads.  *)
+
+            
       (* specialize (IHc1 st1 st'1 st2 st'0 r1).
       specialize (IHc2 st'1 st''1 st'0 st2'). *)
 
@@ -350,6 +700,6 @@ Proof.
     - inversion Hceval1. inversion Hceval2. subst. unfold find_instance in *.
       intros Hsamereads. inversion H. subst; try easy.
         * inversion H8. subst. inversion H3. subst. *)
-Admitted.
+(* Admitted. *)
 
 
